cfrontend/PrintCsyntax.ml
@@ -269,6 +269,10 @@ let rec expr p (prec, e) =
   | Ebuiltin(EF_debug(kind,txt,_),_,args,_) ->
       fprintf p "__builtin_debug@[<hov 1>(%d,%S%a)@]"
         (P.to_int kind) (extern_atom txt) exprlist (false,args)
+  | Ebuiltin(EF_malloc,_,args,_) -> 
+      fprintf p "malloc@[<hov 1>(%a)@]" exprlist (true,args)
+  | Ebuiltin(EF_free,_,args,_) -> 
+      fprintf p "free@[<hov 1>(%a)@]" exprlist (true,args)
   | Ebuiltin(_, _, args, _) ->
       fprintf p "<unknown builtin>@[<hov 1>(%a)@]" exprlist (true, args)
   | Eparen(a1, tycast, ty) ->
